declared some arguments maximally implicit, and started to replace Add [Parametric] Morphism and Add Relation by Instance, and Implicit Arguments by Arguments

Filter/AFilterBool.v
@@ -13,326 +13,322 @@ Require Import ATrs VecFilter VecUtil LogicUtil List RelUtil SN NatUtil.
 
 Section S.
 
-Variable Sig : Signature.
+  Variable Sig : Signature.
 
 (***********************************************************************)
 (** filtering function *)
 
-Variable pi : forall f, bools (@arity Sig f).
+  Variable pi : forall f, bools (@arity Sig f).
 
 (***********************************************************************)
 (** filtered signature *)
 
-Definition filter_arity f := Vtrue (pi f).
+  Definition filter_arity f := Vtrue (pi f).
 
-Definition filter_sig := mkSignature filter_arity (@beq_symb_ok Sig).
-Notation Sig' := filter_sig.
+  Definition filter_sig := mkSignature filter_arity (@beq_symb_ok Sig).
+  Notation Sig' := filter_sig.
 
-Notation term' := (ATerm.term Sig'). Notation Fun' := (@Fun Sig').
-Notation term := (term Sig). Notation terms := (vector term).
+  Notation term' := (ATerm.term Sig'). Notation Fun' := (@Fun Sig').
+  Notation term := (term Sig). Notation terms := (vector term).
 
-Notation context' := (context Sig'). Definition Cont' := (@Cont Sig').
-Notation context := (context Sig).
+  Notation context' := (context Sig'). Definition Cont' := (@Cont Sig').
+  Notation context := (context Sig).
 
 (***********************************************************************)
 (** term filtering *)
 
-Fixpoint filter (t : term) : term' :=
-  match t with
-    | Var x => Var x
-    | Fun f ts => Fun' f (Vfilter (pi f) (Vmap filter ts))
-  end.
+  Fixpoint filter (t : term) : term' :=
+    match t with
+      | Var x => Var x
+      | Fun f ts => Fun' f (Vfilter (pi f) (Vmap filter ts))
+    end.
 
 (***********************************************************************)
 (** rule filtering *)
 
-Notation rule' := (rule Sig'). Notation rules' := (list rule').
-Notation rule := (rule Sig). Notation rules := (list rule).
+  Notation rule' := (rule Sig'). Notation rules' := (list rule').
+  Notation rule := (rule Sig). Notation rules := (list rule).
 
-Definition filter_rule a := mkRule (filter (lhs a)) (filter (rhs a)).
+  Definition filter_rule a := mkRule (filter (lhs a)) (filter (rhs a)).
 
-Notation filter_rules := (List.map filter_rule).
+  Notation filter_rules := (List.map filter_rule).
 
 (***********************************************************************)
 (** properties wrt substitutions *)
 
-Definition filter_subs s (x : variable) := filter (s x).
+  Definition filter_subs s (x : variable) := filter (s x).
 
-Lemma filter_sub : forall s t,
-  filter (sub s t) = sub (filter_subs s) (filter t).
+  Lemma filter_sub : forall s t,
+    filter (sub s t) = sub (filter_subs s) (filter t).
 
-Proof.
-intro. apply term_ind_forall with
-(P := fun t => filter (sub s t) = sub (filter_subs s) (filter t)); intros.
-refl. simpl.
-apply args_eq. repeat rewrite <- Vmap_filter. repeat rewrite Vmap_map.
-apply Vmap_eq. eapply Vforall_incl with (v2 := v). intros.
-eapply Vfilter_in. apply H0. hyp.
-Qed.
+  Proof.
+    intro. apply term_ind_forall with
+    (P := fun t => filter (sub s t) = sub (filter_subs s) (filter t)); intros.
+    refl. simpl.
+    apply args_eq. repeat rewrite <- Vmap_filter. repeat rewrite Vmap_map.
+    apply Vmap_eq. eapply Vforall_incl with (v2 := v). intros.
+    eapply Vfilter_in. apply H0. hyp.
+  Qed.
 
 (***********************************************************************)
 (** filter ordering *)
 
-Section filter_ordering.
+  Section filter_ordering.
 
-Variable succ : relation term'.
+    Variable succ : relation term'.
 
-Definition filter_ord : relation term := fun t u => succ (filter t) (filter u).
+    Definition filter_ord : relation term :=
+      fun t u => succ (filter t) (filter u).
 
-Notation fsucc := filter_ord.
+    Notation fsucc := filter_ord.
 
 (***********************************************************************)
 (** transitivity *)
 
-Lemma filter_trans : transitive succ -> transitive fsucc.
+    Lemma filter_trans : transitive succ -> transitive fsucc.
 
-Proof.
-intro. unfold transitive, filter_ord. intros. eapply H. apply H0. hyp.
-Qed.
+    Proof.
+      intro. unfold transitive, filter_ord. intros. eapply H. apply H0. hyp.
+    Qed.
 
 (***********************************************************************)
 (** well-foundedness *)
 
-Require Import ARelation.
+    Require Import ARelation.
 
-Lemma WF_filter : WF succ -> WF fsucc.
+    Lemma WF_filter : WF succ -> WF fsucc.
 
-Proof.
-intro. unfold filter_ord. apply (WF_inverse filter H).
-Qed.
+    Proof. intro. unfold filter_ord. apply (WF_inverse filter H). Qed.
 
 (***********************************************************************)
 (** stability by substitution *)
 
-Lemma filter_subs_closed :
-  substitution_closed succ -> substitution_closed fsucc.
+    Lemma filter_subs_closed :
+      substitution_closed succ -> substitution_closed fsucc.
 
-Proof.
-unfold substitution_closed. intros. unfold filter_ord.
-repeat rewrite filter_sub. apply H. hyp.
-Qed.
+    Proof.
+      unfold substitution_closed. intros. unfold filter_ord.
+      repeat rewrite filter_sub. apply H. hyp.
+    Qed.
 
 (***********************************************************************)
 (** compatibility *)
 
-Require Import ACompat.
+    Require Import ACompat.
 
-Lemma filter_comp : forall R : rules,
-  compat succ (filter_rules R) -> compat fsucc R.
+    Lemma filter_comp : forall R : rules,
+      compat succ (filter_rules R) -> compat fsucc R.
 
-Proof.
-unfold compat. intros. unfold filter_ord. apply H.
-change (In (filter_rule (mkRule l r)) (filter_rules R)).
-apply in_map. hyp.
-Qed.
+    Proof.
+      unfold compat. intros. unfold filter_ord. apply H.
+      change (In (filter_rule (mkRule l r)) (filter_rules R)).
+      apply in_map. hyp.
+    Qed.
 
 (***********************************************************************)
 (** properties wrt contexts *)
 
-Section filter_cont.
+    Section filter_cont.
 
-Variables (f : Sig) (i j : nat) (e : i + S j = arity f)
-  (v1 : terms i) (c : context) (v2 : terms j) (t : term).
+      Variables (f : Sig) (i j : nat) (e : i + S j = arity f)
+        (v1 : terms i) (c : context) (v2 : terms j) (t : term).
 
-Let bs := Vbreak (n1:=i) (n2:=S j) (Vcast (pi f) (sym_eq e)).
-Let v1' := Vfilter (fst bs) (Vmap filter v1).
-Let t' := filter (fill c t).
-Let v2' := Vfilter (Vtail (snd bs)) (Vmap filter v2).
-Let h := trans_eq (Vtrue_break (n1:=i) (n2:=S j) (Vcast (pi f) (sym_eq e)))
-  (Vtrue_cast (pi f) (sym_eq e)).
+      Let bs := Vbreak (n1:=i) (n2:=S j) (Vcast (pi f) (sym_eq e)).
+      Let v1' := Vfilter (fst bs) (Vmap filter v1).
+      Let t' := filter (fill c t).
+      Let v2' := Vfilter (Vtail (snd bs)) (Vmap filter v2).
+      Let h := trans_eq (Vtrue_break (n1:=i) (n2:=S j)
+        (Vcast (pi f) (sym_eq e))) (Vtrue_cast (pi f) (sym_eq e)).
 
-Section filter_cont_true.
+      Section filter_cont_true.
 
-Variable H : Vhead (snd bs) = true.
+        Variable H : Vhead (snd bs) = true.
 
-Definition e_true := trans_eq (plus_reg_l_inv (Vtrue (fst bs))
-  (Vtrue_Sn_true (snd bs) H)) h.
+        Definition e_true := trans_eq (plus_reg_l_inv (Vtrue (fst bs))
+          (Vtrue_Sn_true (snd bs) H)) h.
 
-Lemma filter_cont_true :
-  filter (fill (Cont f e v1 c v2) t) = fill (Cont' f e_true v1' Hole v2') t'.
+        Lemma filter_cont_true : filter (fill (Cont f e v1 c v2) t)
+          = fill (Cont' f e_true v1' Hole v2') t'.
 
-Proof.
-simpl. rewrite Vmap_cast. rewrite Vmap_app. simpl.
-rewrite Vfilter_cast. rewrite Vfilter_app. rewrite Vcast_cast. fold bs t' v1'.
-assert (Vfilter (snd bs) (Vcons t' (Vmap filter v2))
-  = Vcast (Vcons t' v2') (Vtrue_Sn_true (snd bs) H)).
-rewrite (Vfilter_head_true t' (Vmap filter v2) H). refl. rewrite H0.
-rewrite Vapp_rcast. rewrite Vcast_cast. refl.
-Qed.
+        Proof.
+          simpl. rewrite Vmap_cast, Vmap_app. simpl.
+          rewrite Vfilter_cast, Vfilter_app, Vcast_cast. fold bs t' v1'.
+          assert (Vfilter (snd bs) (Vcons t' (Vmap filter v2))
+            = Vcast (Vcons t' v2') (Vtrue_Sn_true (snd bs) H)).
+          rewrite (Vfilter_head_true t' (Vmap filter v2) H). refl.
+          rewrite H0, Vapp_rcast, Vcast_cast. refl.
+        Qed.
 
-End filter_cont_true.
+      End filter_cont_true.
 
-Section filter_cont_false.
+      Section filter_cont_false.
 
-Variable H : Vhead (snd bs) = false.
+        Variable H : Vhead (snd bs) = false.
 
-Definition e_false := trans_eq (plus_reg_l_inv (Vtrue (fst bs))
-  (Vtrue_Sn_false (snd bs) H)) h.
+        Definition e_false := trans_eq (plus_reg_l_inv (Vtrue (fst bs))
+          (Vtrue_Sn_false (snd bs) H)) h.
 
-Lemma filter_cont_false :
-  filter (fill (Cont f e v1 c v2) t) = Fun' f (Vcast (Vapp v1' v2') e_false).
+        Lemma filter_cont_false : filter (fill (Cont f e v1 c v2) t)
+          = Fun' f (Vcast (Vapp v1' v2') e_false).
 
-Proof.
-simpl. rewrite Vmap_cast. rewrite Vmap_app. simpl.
-rewrite Vfilter_cast. rewrite Vfilter_app. rewrite Vcast_cast. fold bs t' v1'.
-assert (Vfilter (snd bs) (Vcons t' (Vmap filter v2))
-  = Vcast v2' (Vtrue_Sn_false (snd bs) H)).
-rewrite (Vfilter_head_false t' (Vmap filter v2) H). refl. rewrite H0.
-rewrite Vapp_rcast. rewrite Vcast_cast. refl.
-Qed.
+        Proof.
+          simpl. rewrite Vmap_cast, Vmap_app. simpl.
+          rewrite Vfilter_cast, Vfilter_app, Vcast_cast. fold bs t' v1'.
+          assert (Vfilter (snd bs) (Vcons t' (Vmap filter v2))
+            = Vcast v2' (Vtrue_Sn_false (snd bs) H)).
+          rewrite (Vfilter_head_false t' (Vmap filter v2) H). refl.
+          rewrite H0, Vapp_rcast, Vcast_cast. refl.
+        Qed.
 
-End filter_cont_false.
+      End filter_cont_false.
 
-End filter_cont.
+    End filter_cont.
 
-Implicit Arguments filter_cont_true [f i j].
-Implicit Arguments filter_cont_false [f i j].
+    Implicit Arguments filter_cont_true [f i j].
+    Implicit Arguments filter_cont_false [f i j].
 
 (***********************************************************************)
 (** stability wrt contexts *)
 
-Lemma filter_cont_closed :
-  reflexive succ -> context_closed succ -> context_closed fsucc.
+    Lemma filter_cont_closed :
+      reflexive succ -> context_closed succ -> context_closed fsucc.
 
-Proof.
-intros Hrefl H. unfold context_closed, filter_ord. induction c; intros.
-simpl. hyp.
-set (bs := Vbreak (n1:=i) (n2:=S j) (Vcast (pi f) (sym_eq e))).
-case_eq (Vhead (snd bs)); intro H1.
-rewrite (filter_cont_true e t c t0 t1 H1).
-rewrite (filter_cont_true e t c t0 t2 H1). apply H. apply IHc. hyp.
-rewrite (filter_cont_false e t c t0 t1 H1).
-rewrite (filter_cont_false e t c t0 t2 H1). apply Hrefl.
-Qed.
+    Proof.
+      intros Hrefl H. unfold context_closed, filter_ord. induction c; intros.
+      simpl. hyp.
+      set (bs := Vbreak (n1:=i) (n2:=S j) (Vcast (pi f) (sym_eq e))).
+      case_eq (Vhead (snd bs)); intro H1.
+      rewrite (filter_cont_true e t c t0 t1 H1).
+      rewrite (filter_cont_true e t c t0 t2 H1). apply H. apply IHc. hyp.
+      rewrite (filter_cont_false e t c t0 t1 H1).
+      rewrite (filter_cont_false e t c t0 t2 H1). apply Hrefl.
+    Qed.
 
-End filter_ordering.
+  End filter_ordering.
 
 (***********************************************************************)
 (** monotony wrt inclusion *)
 
-Lemma incl_filter : forall R S, R << S -> filter_ord R << filter_ord S.
+  Lemma incl_filter : forall R S, R << S -> filter_ord R << filter_ord S.
 
-Proof.
-intros. unfold inclusion, filter_ord. intros. apply H. exact H0.
-Qed.
+  Proof. intros. unfold inclusion, filter_ord. intros. apply H. exact H0. Qed.
 
 (***********************************************************************)
 (** weak stability wrt contexts *)
 
-Section weak_cont_closed.
+  Section weak_cont_closed.
 
-Variable succ : relation term'.
-Notation fsucc := (filter_ord succ).
-Notation succ_eq := (clos_refl succ).
-Notation fsucc_eq := (filter_ord succ_eq).
+    Variable succ : relation term'.
 
-Lemma filter_ord_rc : reflexive fsucc_eq.
+    Notation fsucc := (filter_ord succ).
+    Notation succ_eq := (clos_refl succ).
+    Notation fsucc_eq := (filter_ord succ_eq).
 
-Proof.
-unfold reflexive, filter_ord, clos_refl, union. auto.
-Qed.
+    Lemma filter_ord_rc : reflexive fsucc_eq.
 
-Lemma rc_filter_ord : inclusion (clos_refl fsucc) fsucc_eq.
+    Proof. unfold reflexive, filter_ord, clos_refl, union. auto. Qed.
 
-Proof.
-unfold inclusion, clos_refl, union, filter_ord.
-intros. decomp H. subst y. auto. auto.
-Qed.
+    Lemma rc_filter_ord : inclusion (clos_refl fsucc) fsucc_eq.
 
-Lemma filter_weak_cont_closed :
-  weak_context_closed succ succ_eq -> weak_context_closed fsucc fsucc_eq.
+    Proof.
+      unfold inclusion, clos_refl, union, filter_ord.
+      intros. decomp H. subst y. auto. auto.
+    Qed.
 
-Proof.
-intro. unfold weak_context_closed. intros.
-assert (clos_refl fsucc t1 t2). unfold clos_refl, union. auto.
-ded (rc_filter_ord H1).
-assert (context_closed fsucc_eq). apply filter_cont_closed. apply rc_refl.
-apply rc_context_closed. hyp. apply H3. hyp.
-Qed.
+    Lemma filter_weak_cont_closed :
+      weak_context_closed succ succ_eq -> weak_context_closed fsucc fsucc_eq.
+
+    Proof.
+      intro. unfold weak_context_closed. intros.
+      assert (clos_refl fsucc t1 t2). unfold clos_refl, union. auto.
+      ded (rc_filter_ord H1).
+      assert (context_closed fsucc_eq). apply filter_cont_closed. apply rc_refl.
+      apply rc_context_closed. hyp. apply H3. hyp.
+    Qed.
 
 (***********************************************************************)
 (** reduction ordering *)
 
-Lemma filter_weak_red_ord : weak_reduction_ordering succ succ_eq
-  -> weak_reduction_ordering fsucc fsucc_eq.
+    Lemma filter_weak_red_ord : weak_reduction_ordering succ succ_eq
+      -> weak_reduction_ordering fsucc fsucc_eq.
 
-Proof.
-intro. destruct H as [Hwf (Hsubs,Hcont)]. split. apply WF_filter. hyp.
-split. apply filter_subs_closed. hyp.
-apply filter_weak_cont_closed. hyp.
-Qed.
+    Proof.
+      intro. destruct H as [Hwf (Hsubs,Hcont)]. split. apply WF_filter. hyp.
+      split. apply filter_subs_closed. hyp.
+      apply filter_weak_cont_closed. hyp.
+    Qed.
 
-End weak_cont_closed.
+  End weak_cont_closed.
 
 (***********************************************************************)
 (** rewriting *)
 
-Section red.
+  Section red.
 
-Variable R : rules.
-Notation R' := (filter_rules R).
+    Variable R : rules.
+    Notation R' := (filter_rules R).
 
-Lemma red_incl_filter_red_rc : red R << filter_ord (red R' %).
+    Lemma red_incl_filter_red_rc : red R << filter_ord (red R' %).
 
-Proof.
-unfold inclusion, filter_ord. intros. redtac. subst x. subst y.
-elim c. simpl. right. repeat rewrite filter_sub. apply red_rule_top.
-change (In (filter_rule (mkRule l r)) R'). apply in_map. hyp.
-intros. set (bs := Vbreak (n1:=i) (n2:=S j) (Vcast (pi f) (sym_eq e))).
-case_eq (Vhead (snd bs)); intro H0.
-rewrite (filter_cont_true f e t c0 t0 (sub s l) H0).
-rewrite (filter_cont_true f e t c0 t0 (sub s r) H0). fold bs. destruct H.
-left. simpl fill. rewrite H. refl. right. apply red_fill. hyp.
-left. rewrite (filter_cont_false f e t c0 t0 (sub s l) H0).
-rewrite (filter_cont_false f e t c0 t0 (sub s r) H0). refl.
-Qed.
+    Proof.
+      unfold inclusion, filter_ord. intros. redtac. subst x. subst y.
+      elim c. simpl. right. repeat rewrite filter_sub. apply red_rule_top.
+      change (In (filter_rule (mkRule l r)) R'). apply in_map. hyp.
+      intros. set (bs := Vbreak (n1:=i) (n2:=S j) (Vcast (pi f) (sym_eq e))).
+      case_eq (Vhead (snd bs)); intro H0.
+      rewrite (filter_cont_true f e t c0 t0 (sub s l) H0).
+      rewrite (filter_cont_true f e t c0 t0 (sub s r) H0). fold bs. destruct H.
+      left. simpl fill. rewrite H. refl. right. apply red_fill. hyp.
+      left. rewrite (filter_cont_false f e t c0 t0 (sub s l) H0).
+      rewrite (filter_cont_false f e t c0 t0 (sub s r) H0). refl.
+    Qed.
 
-Lemma red_rtc_incl_filter_red_rtc : red R # << filter_ord (red R' #).
+    Lemma red_rtc_incl_filter_red_rtc : red R # << filter_ord (red R' #).
 
-Proof.
-unfold inclusion. induction 1.
-apply incl_filter with (red R' %). apply rc_incl_rtc.
-apply red_incl_filter_red_rc. exact H.
-unfold filter_ord. apply rt_refl.
-unfold filter_ord. apply rt_trans with (filter y).
-apply IHclos_refl_trans1. apply IHclos_refl_trans2.
-Qed.
+    Proof.
+      unfold inclusion. induction 1.
+      apply incl_filter with (red R' %). apply rc_incl_rtc.
+      apply red_incl_filter_red_rc. exact H.
+      unfold filter_ord. apply rt_refl.
+      unfold filter_ord. apply rt_trans with (filter y).
+      apply IHclos_refl_trans1. apply IHclos_refl_trans2.
+    Qed.
 
-Lemma hd_red_incl_filter_hd_red : hd_red R << filter_ord (hd_red R').
+    Lemma hd_red_incl_filter_hd_red : hd_red R << filter_ord (hd_red R').
 
-Proof.
-unfold inclusion, filter_ord. intros. redtac. subst x. subst y.
-repeat rewrite filter_sub. apply hd_red_rule.
-change (In (filter_rule (mkRule l r)) R'). apply in_map. hyp.
-Qed.
+    Proof.
+      unfold inclusion, filter_ord. intros. redtac. subst x. subst y.
+      repeat rewrite filter_sub. apply hd_red_rule.
+      change (In (filter_rule (mkRule l r)) R'). apply in_map. hyp.
+    Qed.
 
-End red.
+  End red.
 
 (***********************************************************************)
 (** rewriting modulo *)
 
-Section red_mod.
+  Section red_mod.
 
-Variable E R : rules.
-Notation E' := (filter_rules E).
-Notation R' := (filter_rules R).
+    Variable E R : rules.
+    Notation E' := (filter_rules E).
+    Notation R' := (filter_rules R).
 
-Lemma hd_red_mod_filter : hd_red_mod E R << filter_ord (hd_red_mod E' R').
+    Lemma hd_red_mod_filter : hd_red_mod E R << filter_ord (hd_red_mod E' R').
 
-Proof.
-unfold inclusion, filter_ord. intros. redtac. exists (filter t). split.
-apply red_rtc_incl_filter_red_rtc. exact H.
-subst t. subst y. repeat rewrite filter_sub. apply hd_red_rule.
-change (In (filter_rule (mkRule l r)) R'). apply in_map. hyp.
-Qed.
+    Proof.
+      unfold inclusion, filter_ord. intros. redtac. exists (filter t). split.
+      apply red_rtc_incl_filter_red_rtc. exact H.
+      subst t. subst y. repeat rewrite filter_sub. apply hd_red_rule.
+      change (In (filter_rule (mkRule l r)) R'). apply in_map. hyp.
+    Qed.
 
-Lemma WF_hd_red_mod_filter : WF (hd_red_mod E' R') -> WF (hd_red_mod E R).
+    Lemma WF_hd_red_mod_filter : WF (hd_red_mod E' R') -> WF (hd_red_mod E R).
 
-Proof.
-intro. eapply WF_incl. apply hd_red_mod_filter. apply WF_filter. hyp.
-Qed.
+    Proof.
+      intro. eapply WF_incl. apply hd_red_mod_filter. apply WF_filter. hyp.
+    Qed.
 
-End red_mod.
+  End red_mod.
 
 End S.
 
