Term/WithArity/ARules.v
@@ -13,45 +13,42 @@ Require Import ATrs ListUtil RelUtil ARelation LogicUtil SetUtil.
 
 Section defs.
 
-Variable Sig : Signature.
+  Variable Sig : Signature.
 
-Notation term := (term Sig). Notation rule := (rule Sig).
+  Notation term := (term Sig). Notation rule := (rule Sig).
 
-Definition rules := set rule.
+  Definition rules := set rule.
 
 (***********************************************************************)
 (** finite rewriting *)
 
-Definition Rules R : rules := fun x => In x R.
+  Definition Rules R : rules := fun x => In x R.
 
-Lemma Rules_cons : forall a R, Rules (a :: R) [=] a :: Rules R.
+  Lemma Rules_cons : forall a R, Rules (a :: R) [=] a :: Rules R.
 
-Proof.
-unfold Rules. simpl. split. intuition. subst. fo. fo.
-fo.
-Qed.
+  Proof. unfold Rules. simpl. split. intuition. subst. fo. fo. fo. Qed.
 
-Lemma Rules_app : forall R S, Rules (R ++ S) [=] Rules R ++ Rules S.
+  Lemma Rules_app : forall R S, Rules (R ++ S) [=] Rules R ++ Rules S.
 
-Proof.
-split; unfold Rules, union; intro. rewrite in_app in H. hyp. destruct H.
-apply in_appl. hyp. apply in_appr. hyp.
-Qed.
+  Proof.
+    split; unfold Rules, union; intro. rewrite in_app in H. hyp. destruct H.
+    apply in_appl. hyp. apply in_appr. hyp.
+  Qed.
 
 (***********************************************************************)
 (** rewriting *)
 
-Definition red (R : rules) : relation term :=
-  fun u v => exists l, exists r, exists c, exists s,
-    R (mkRule l r) /\ u = fill c (sub s l) /\ v = fill c (sub s r).
+  Definition red (R : rules) : relation term :=
+    fun u v => exists l, exists r, exists c, exists s,
+      R (mkRule l r) /\ u = fill c (sub s l) /\ v = fill c (sub s r).
 
-Definition hd_red (R : rules) : relation term :=
-  fun u v => exists l, exists r, exists s,
-    R (mkRule l r) /\ u = sub s l /\ v = sub s r.
+  Definition hd_red (R : rules) : relation term :=
+    fun u v => exists l, exists r, exists s,
+      R (mkRule l r) /\ u = sub s l /\ v = sub s r.
 
-Definition red_mod E R := red E # @ red R.
+  Definition red_mod E R := red E # @ red R.
 
-Definition hd_red_mod E R := red E # @ hd_red R.
+  Definition hd_red_mod E R := red E # @ hd_red R.
 
 End defs.
 
@@ -94,7 +91,7 @@ apply RR'. hyp.
 Qed.
 
 Add Parametric Morphism (Sig : Signature) : (@red Sig)
-  with signature (@SetUtil.equiv (@rule Sig)) ==> (same_relation (term Sig))
+  with signature (@SetUtil.equiv (@rule Sig)) ==> (@same_relation (term Sig))
     as red_equiv.
 
 Proof.
@@ -122,7 +119,7 @@ apply RR'. hyp.
 Qed.
 
 Add Parametric Morphism (Sig : Signature) : (@hd_red Sig)
-  with signature (@SetUtil.equiv (@rule Sig)) ==> (same_relation (term Sig))
+  with signature (@SetUtil.equiv (@rule Sig)) ==> (@same_relation (term Sig))
     as hd_red_equiv.
 
 Proof.
@@ -150,7 +147,7 @@ Qed.
 
 Add Parametric Morphism (Sig : Signature) : (@red_mod Sig)
   with signature (@SetUtil.equiv (@rule Sig)) ==>
-    (@SetUtil.equiv (@rule Sig)) ==> (same_relation (term Sig))
+    (@SetUtil.equiv (@rule Sig)) ==> (@same_relation (term Sig))
     as red_mod_equiv.
 
 Proof.
@@ -183,7 +180,7 @@ Qed.
 
 Add Parametric Morphism (Sig : Signature) : (@hd_red_mod Sig)
   with signature (@SetUtil.equiv (@rule Sig)) ==>
-    (@SetUtil.equiv (@rule Sig)) ==> (same_relation (term Sig))
+    (@SetUtil.equiv (@rule Sig)) ==> (@same_relation (term Sig))
     as hd_red_mod_equiv.
 
 Proof.
@@ -209,105 +206,101 @@ Qed.
 
 Section props.
 
-Variable Sig : Signature.
+  Variable Sig : Signature.
 
-Notation rule := (rule Sig). Notation rules := (set rule).
-Notation Rules := (@Rules Sig). Notation empty := (@empty rule).
+  Notation rule := (rule Sig). Notation rules := (set rule).
+  Notation Rules := (@Rules Sig).
 
-Lemma red_rule : forall (R : rules) l r c s, R (mkRule l r) ->
-  red R (fill c (sub s l)) (fill c (sub s r)).
+  Lemma red_rule : forall (R : rules) l r c s, R (mkRule l r) ->
+    red R (fill c (sub s l)) (fill c (sub s r)).
 
-Proof.
-intros. unfold red. exists l. exists r. exists c. exists s. auto.
-Qed.
+  Proof. intros. unfold red. exists l. exists r. exists c. exists s. auto. Qed.
 
-Lemma hd_red_rule : forall (R : rules) l r s, R (mkRule l r) ->
-  hd_red R (sub s l) (sub s r).
+  Lemma hd_red_rule : forall (R : rules) l r s, R (mkRule l r) ->
+    hd_red R (sub s l) (sub s r).
 
-Proof.
-intros. unfold hd_red. exists l. exists r. exists s. auto.
-Qed.
+  Proof. intros. unfold hd_red. exists l. exists r. exists s. auto. Qed.
 
-Lemma context_closed_red : forall R : rules, context_closed (red R).
+  Lemma context_closed_red : forall R : rules, context_closed (red R).
 
-Proof.
-intros R t u c h. redtac. subst. repeat rewrite fill_fill.
-exists l. exists r. exists (comp c c0). exists s. intuition.
-Qed.
+  Proof.
+    intros R t u c h. redtac. subst. repeat rewrite fill_fill.
+    exists l. exists r. exists (comp c c0). exists s. intuition.
+  Qed.
 
-Lemma red_Rules : forall R, red (Rules R) == ATrs.red R.
+  Lemma red_Rules : forall R, red (Rules R) == ATrs.red R.
 
-Proof.
-split; intros t u H. redtac. subst. apply ATrs.red_rule. hyp.
-ATrs.redtac. subst. apply red_rule. hyp.
-Qed.
+  Proof.
+    split; intros t u H. redtac. subst. apply ATrs.red_rule. hyp.
+    ATrs.redtac. subst. apply red_rule. hyp.
+  Qed.
 
-Lemma hd_red_Rules : forall R, hd_red (Rules R) == ATrs.hd_red R.
+  Lemma hd_red_Rules : forall R, hd_red (Rules R) == ATrs.hd_red R.
 
-Proof.
-split; intros t u H. redtac. subst. apply ATrs.hd_red_rule. hyp.
-ATrs.redtac. subst. apply hd_red_rule. hyp.
-Qed.
+  Proof.
+    split; intros t u H. redtac. subst. apply ATrs.hd_red_rule. hyp.
+    ATrs.redtac. subst. apply hd_red_rule. hyp.
+  Qed.
 
-Lemma rt_red_empty : red empty # == @eq (@term Sig).
+  Lemma rt_red_empty : red (@empty rule) # == eq.
 
-Proof.
-split; intros t u h. elim h; intros. redtac. contr. refl.
-trans y; hyp. subst. apply rt_refl.
-Qed.
+  Proof.
+    split; intros t u h. elim h; intros. redtac. contr. refl.
+    trans y; hyp. subst. apply rt_refl.
+  Qed.
 
 (***********************************************************************)
 (** properties of rewriting modulo *)
 
-Lemma context_closed_red_mod : forall E R : rules,
-  context_closed (red_mod E R).
+  Lemma context_closed_red_mod : forall E R : rules,
+    context_closed (red_mod E R).
 
-Proof.
-intros. apply context_closed_comp. apply context_closed_rtc.
-apply context_closed_red. apply context_closed_red.
-Qed.
+  Proof.
+    intros. apply context_closed_comp. apply context_closed_rtc.
+    apply context_closed_red. apply context_closed_red.
+  Qed.
 
-Lemma red_mod_union : forall E R : rules, red_mod E R << red (E ++ R) #.
+  Lemma red_mod_union : forall E R : rules, red_mod E R << red (E ++ R) #.
 
-Proof.
-intros E R t u [h [h1 h2]]. revert h1 h2. induction 1; intro.
-apply rt_trans with y.
-apply rt_step. apply red_incl with E. apply incl_appl. hyp.
-apply rt_step. apply red_incl with R. apply incl_appr. hyp.
-apply rt_step. apply red_incl with R. apply incl_appr. hyp.
-apply rt_trans with y.
-eapply inclusion_elim. apply clos_refl_trans_m'. apply red_incl.
-apply incl_appl. hyp.
-auto.
-Qed.
+  Proof.
+    intros E R t u [h [h1 h2]]. revert h1 h2. induction 1; intro.
+    apply rt_trans with y.
+    apply rt_step. apply red_incl with E. apply incl_appl. hyp.
+    apply rt_step. apply red_incl with R. apply incl_appr. hyp.
+    apply rt_step. apply red_incl with R. apply incl_appr. hyp.
+    apply rt_trans with y.
+    eapply inclusion_elim. apply clos_refl_trans_m'. apply red_incl.
+    apply incl_appl. hyp.
+    auto.
+  Qed.
 
-Lemma rt_red_mod_union : forall E R : rules, red_mod E R # << red (E ++ R) #.
+  Lemma rt_red_mod_union : forall E R : rules, red_mod E R # << red (E ++ R) #.
 
-Proof.
-intros. incl_trans (red(E++R)##). rewrite red_mod_union. refl.
-rewrite rtc_invol. refl.
-Qed.
+  Proof.
+    intros. incl_trans (red(E++R)##). rewrite red_mod_union. refl.
+    rewrite rtc_invol. refl.
+  Qed.
 
-Lemma red_mod_Rules : forall E R,
-  red_mod (Rules E) (Rules R) == ATrs.red_mod E R.
+  Lemma red_mod_Rules : forall E R,
+    red_mod (Rules E) (Rules R) == ATrs.red_mod E R.
 
-Proof.
-intros. unfold red_mod, ATrs.red_mod. repeat rewrite red_Rules. refl.
-Qed.
+  Proof.
+    intros. unfold red_mod, ATrs.red_mod. repeat rewrite red_Rules. refl.
+  Qed.
 
-Lemma hd_red_mod_Rules : forall E R,
-  hd_red_mod (Rules E) (Rules R) == ATrs.hd_red_mod E R.
+  Lemma hd_red_mod_Rules : forall E R,
+    hd_red_mod (Rules E) (Rules R) == ATrs.hd_red_mod E R.
 
-Proof.
-intros. unfold hd_red_mod, ATrs.hd_red_mod. repeat rewrite red_Rules.
-repeat rewrite hd_red_Rules. refl.
-Qed.
+  Proof.
+    intros. unfold hd_red_mod, ATrs.hd_red_mod. repeat rewrite red_Rules.
+    repeat rewrite hd_red_Rules. refl.
+  Qed.
 
-Lemma red_mod_empty : forall R : rules, red_mod empty R == red R.
+  Lemma red_mod_empty : forall R : rules, red_mod (@empty rule) R == red R.
 
-Proof.
-intro. unfold red_mod. rewrite rt_red_empty. split; intros t u h.
-destruct h. intuition. subst. hyp. exists t. auto.
-Qed.
+  Proof.
+    intro. unfold red_mod. rewrite rt_red_empty. split; intros t u h.
+    destruct h. intuition. subst. hyp. exists t. auto.
+  Qed.
 
 End props.
