Util/Nat/BoundNat.v
@@ -13,137 +13,138 @@ Require Import NatUtil LogicUtil Multiset Permutation PermutSetoid.
 
 Section S.
 
-Variable dim : nat.
+  Variable dim : nat.
 
-(*FIXME: use NatUtil.nat_lt instead*)
+  (*FIXME: use NatUtil.nat_lt instead*)
 
-Definition bnat := {x : nat | x < dim}. 
+  Definition bnat := {x : nat | x < dim}. 
 
-Definition mkbnat x (h : x<dim) := exist (fun x => x<dim) x h.
+  Definition mkbnat x (h : x<dim) := exist (fun x => x<dim) x h.
 
-Lemma eq_bnat_dec : forall x y : bnat, {x = y} + {x <> y}.
+  Lemma eq_bnat_dec : forall x y : bnat, {x = y} + {x <> y}.
 
-Proof.
-intros.
-destruct (eq_nat_dec (proj1_sig x) (proj1_sig y)); unfold proj1_sig in *.
-destruct x. destruct y. subst; simpl. left.
-cut (l=l0). intro; subst. intuition. apply lt_unique.
-destruct x. destruct y. right; intuition; inversion H; tauto.
-Defined.
+  Proof.
+    intros.
+    destruct (eq_nat_dec (proj1_sig x) (proj1_sig y)); unfold proj1_sig in *.
+    destruct x. destruct y. subst; simpl. left.
+    cut (l=l0). intro; subst. intuition. apply lt_unique.
+    destruct x. destruct y. right; intuition; inversion H; tauto.
+  Defined.
 
-Lemma bnat_spec : forall x, x < dim <-> exists y : bnat, proj1_sig y = x.
+  Lemma bnat_spec : forall x, x < dim <-> exists y : bnat, proj1_sig y = x.
 
-Proof.
-split; intro.
-Focus 2. destruct H. destruct x0. simpl in *. intuition.
-exists (mkbnat H). simpl. refl.
-Qed.
+  Proof.
+    split; intro.
+    Focus 2. destruct H. destruct x0. simpl in *. intuition.
+    exists (mkbnat H). simpl. refl.
+  Qed.
 
-Require Import ListExtras.
+  Require Import ListExtras.
 
-Fixpoint bnats_of_nats l :=
-  match l with
-    | nil => nil
-    | x::q =>
-      match lt_ge_dec x dim with 
-        | left H => mkbnat H :: bnats_of_nats q
-        | right _ => bnats_of_nats q
-     end
-  end.
+  Fixpoint bnats_of_nats l :=
+    match l with
+      | nil => nil
+      | x::q =>
+        match lt_ge_dec x dim with 
+          | left H => mkbnat H :: bnats_of_nats q
+          | right _ => bnats_of_nats q
+        end
+    end.
 
-Lemma bnats_of_nats_spec : forall x l (H : x<dim),
-  In x l -> In (mkbnat H) (bnats_of_nats l).
+  Lemma bnats_of_nats_spec : forall x l (H : x<dim),
+    In x l -> In (mkbnat H) (bnats_of_nats l).
 
-Proof.
-intros. induction l. simpl in H0; tauto.
-simpl. destruct(lt_ge_dec a dim). simpl. simpl in H0; destruct H0. subst.
-left. ded (lt_unique l0 H); subst; auto.
-right; tauto.
-simpl in H0; destruct H0. subst. cut False; try tauto; try omega.
-tauto.
-Qed.
+  Proof.
+    intros. induction l. simpl in H0; tauto.
+    simpl. destruct(lt_ge_dec a dim). simpl. simpl in H0; destruct H0. subst.
+    left. ded (lt_unique l0 H); subst; auto.
+    right; tauto.
+    simpl in H0; destruct H0. subst. cut False; try tauto; try omega.
+    tauto.
+  Qed.
 
-Definition nfirst_bnats := bnats_of_nats (nfirst dim).
+  Definition nfirst_bnats := bnats_of_nats (nfirst dim).
 
-Lemma bnatlist_exact : forall x, In x nfirst_bnats.
+  Lemma bnatlist_exact : forall x, In x nfirst_bnats.
 
-Proof.
-intros. unfold nfirst_bnats. destruct x. fold (mkbnat l).
-apply bnats_of_nats_spec. rewrite nfirst_exact. auto.
-Qed.
+  Proof.
+    intros. unfold nfirst_bnats. destruct x. fold (mkbnat l).
+    apply bnats_of_nats_spec. rewrite nfirst_exact. auto.
+  Qed.
 
-Require Import SortUtil.
+  Require Import SortUtil.
 
-Lemma map_lelistA_bnat_to_nat : forall R (a : bnat) l,
-  lelistA (fun x y => R (proj1_sig x) (proj1_sig y)) a l ->
-  lelistA R (proj1_sig a) (map (fun y => proj1_sig y) l).
+  Lemma map_lelistA_bnat_to_nat : forall R (a : bnat) l,
+    lelistA (fun x y => R (proj1_sig x) (proj1_sig y)) a l ->
+    lelistA R (proj1_sig a) (map (fun y => proj1_sig y) l).
 
-Proof.
-induction l; intros. simpl; apply nil_leA.
-simpl. inversion H; subst. apply cons_leA; auto.
-Qed.
+  Proof.
+    induction l; intros. simpl; apply nil_leA.
+    simpl. inversion H; subst. apply cons_leA; auto.
+  Qed.
 
-Lemma map_sort_bnat_to_nat : forall R l,
-  sort (fun x y : bnat => R (proj1_sig x) (proj1_sig y)) l ->
-  sort R (map (fun y : bnat => proj1_sig y) l).
+  Lemma map_sort_bnat_to_nat : forall R l,
+    sort (fun x y : bnat => R (proj1_sig x) (proj1_sig y)) l ->
+    sort R (map (fun y : bnat => proj1_sig y) l).
 
-Proof.
-induction l; intros. simpl; apply nil_sort.
-simpl. inversion H; apply cons_sort; try tauto.
-apply map_lelistA_bnat_to_nat. intuition.
-Qed.
+  Proof.
+    induction l; intros. simpl; apply nil_sort.
+    simpl. inversion H; apply cons_sort; try tauto.
+    apply map_lelistA_bnat_to_nat. intuition.
+  Qed.
 
-Lemma nfirst_multiplicity : forall n i,
-  multiplicity (list_contents (@eq nat) eq_nat_dec (nfirst n)) i
-  = if lt_ge_dec i n then 1 else 0.
+  Lemma nfirst_multiplicity : forall n i,
+    multiplicity (list_contents (@eq nat) eq_nat_dec (nfirst n)) i
+    = if lt_ge_dec i n then 1 else 0.
 
-Proof. 
-induction n; intros. simpl. destruct (lt_ge_dec i 0); omega.
-simpl. rewrite IHn. destruct (lt_ge_dec i n); destruct (eq_nat_dec n i);
-destruct (lt_ge_dec i (S n)); try omega.
-Qed.
+  Proof. 
+    induction n; intros. simpl. destruct (lt_ge_dec i 0); omega.
+    simpl. rewrite IHn. destruct (lt_ge_dec i n); destruct (eq_nat_dec n i);
+    destruct (lt_ge_dec i (S n)); try omega.
+  Qed.
 
-Lemma bnfirst_multiplicity n (i : bnat) :
-  multiplicity
-  (list_contents (@eq bnat) eq_bnat_dec (bnats_of_nats (nfirst n))) i
-  = if lt_ge_dec (proj1_sig i) n then 1 else 0.
+  Lemma bnfirst_multiplicity n (i : bnat) :
+    multiplicity
+    (list_contents (@eq bnat) eq_bnat_dec (bnats_of_nats (nfirst n))) i
+    = if lt_ge_dec (proj1_sig i) n then 1 else 0.
 
-Proof.
-destruct i as [i hi]. fold (mkbnat hi). simpl. induction n.
-simpl. destruct (lt_ge_dec i 0); omega.
-simpl. destruct (lt_ge_dec n dim); simpl; rewrite IHn; destruct(eq_nat_dec n i);
-destruct(lt_ge_dec i n); destruct(lt_ge_dec i (S n)); subst; simpl; try omega;
-try congruence.
-destruct (eq_bnat_dec (mkbnat l) (mkbnat hi)); try omega.
-ded (lt_unique l hi); subst; congruence.
-destruct (eq_bnat_dec (mkbnat l) (mkbnat hi)); try omega.
-unfold mkbnat in * |-; congruence.
-destruct (eq_bnat_dec (mkbnat l) (mkbnat hi)); try omega.
-unfold mkbnat in * |-; congruence.
-Qed.
+  Proof.
+    destruct i as [i hi]. fold (mkbnat hi). simpl. induction n.
+    simpl. destruct (lt_ge_dec i 0); omega.
+    simpl. destruct (lt_ge_dec n dim); simpl; rewrite IHn;
+    destruct(eq_nat_dec n i); destruct(lt_ge_dec i n);
+      destruct(lt_ge_dec i (S n)); subst; simpl; try omega;
+        try congruence.
+    destruct (eq_bnat_dec (mkbnat l) (mkbnat hi)); try omega.
+    ded (lt_unique l hi); subst; congruence.
+    destruct (eq_bnat_dec (mkbnat l) (mkbnat hi)); try omega.
+    unfold mkbnat in * |-; congruence.
+    destruct (eq_bnat_dec (mkbnat l) (mkbnat hi)); try omega.
+    unfold mkbnat in * |-; congruence.
+  Qed.
 
-Lemma map_multiplicity : forall a (h : a<dim) mb,
-  multiplicity (list_contents (@eq bnat) eq_bnat_dec mb) (mkbnat h)
-  = multiplicity (list_contents (@eq nat) eq_nat_dec
-    (map (fun y : bnat => proj1_sig y) mb)) a.
+  Lemma map_multiplicity : forall a (h : a<dim) mb,
+    multiplicity (list_contents (@eq bnat) eq_bnat_dec mb) (mkbnat h)
+    = multiplicity (list_contents (@eq nat) eq_nat_dec
+      (map (fun y : bnat => proj1_sig y) mb)) a.
 
-Proof.
-induction mb. simpl; auto.
-simpl. rewrite IHmb. destruct (eq_nat_dec (proj1_sig a0) a);
-destruct (eq_bnat_dec a0 (mkbnat h)); try omega; try congruence.
-destruct a0. simpl in *. subst. ded (lt_unique h l).
-unfold mkbnat in n. congruence.
-destruct a0. simpl in *. unfold mkbnat in e. congruence.
-Qed.
+  Proof.
+    induction mb. simpl; auto.
+    simpl. rewrite IHmb. destruct (eq_nat_dec (proj1_sig a0) a);
+    destruct (eq_bnat_dec a0 (mkbnat h)); try omega; try congruence.
+    destruct a0. simpl in *. subst. ded (lt_unique h l).
+    unfold mkbnat in n. congruence.
+    destruct a0. simpl in *. unfold mkbnat in e. congruence.
+  Qed.
 
-Lemma lemme_foo : forall a (H:a>=dim) mb, 
-  multiplicity (list_contents (eq (A:=nat)) eq_nat_dec
-    (map (fun y : bnat => proj1_sig y) mb)) a = 0.
+  Lemma lemme_foo : forall a (H:a>=dim) mb, 
+    multiplicity (list_contents (eq (A:=nat)) eq_nat_dec
+      (map (fun y : bnat => proj1_sig y) mb)) a = 0.
 
-Proof.
-induction mb. simpl; auto.
-simpl. destruct(eq_nat_dec (proj1_sig a0) a).
-destruct a0; simpl in *; subst; omega. simpl. apply IHmb.
-Qed.
+  Proof.
+    induction mb. simpl; auto.
+    simpl. destruct(eq_nat_dec (proj1_sig a0) a).
+    destruct a0; simpl in *; subst; omega. simpl. apply IHmb.
+  Qed.
 
 End S.
