Util/Relation/Path.v
@@ -87,7 +87,7 @@ Section S.
     assert (incl x0 (a :: l)). apply incl_tl. tauto.
     tauto. exists (a::x0). simpl.
     assert (S (length x0) <= S (length l)). omega. 
-    assert (incl (a :: x0) (a :: l)). apply incl_double_cons. refl. tauto.
+    assert (incl (a :: x0) (a :: l)). apply cons_incl. refl. tauto.
     assert (a<>x). intro. rewrite H7 in H4. tauto.
     assert (a<>y). intro. rewrite H8 in H2. tauto. tauto.
   Qed.
